Get rid of triangular diagrams
With the right setup the rectangular diagrams are as easy to prove,
but they simplify the calling convention algebra significantly when
compared to the triangular diagrams.

cfrontend/Cminorgenproof.v
@@ -148,7 +148,7 @@ Proof.
 Qed.
 
 Section WITHMEMINIT.
-Variable init_nb: block.
+Variable init_f: meminj.
 
 (** * Correspondence between C#minor's and Cminor's environments and memory states *)
 
@@ -424,19 +424,18 @@ Qed.
 (** Global environments match if the memory injection [f] leaves unchanged
   the references to global symbols and functions. *)
 
-Inductive match_globalenvs (f: meminj) (bound: block): Prop :=
+Inductive match_globalenvs (f: meminj): Prop :=
   | mk_match_globalenvs
-      (INIT: Block.le Block.init init_nb)
-      (NEXT: Block.le init_nb bound)
-      (DOMAIN: forall b, Block.lt b bound -> f b = Some(b, 0))
-      (IMAGE: forall b1 b2 delta, f b1 = Some(b2, delta) -> Block.lt b2 bound -> b1 = b2)
-      (SYMBOLS: forall id b, Genv.find_symbol ge id = Some b -> Block.lt b bound)
-      (FUNCTIONS: forall b fd, Genv.find_funct_ptr ge b = Some fd -> Block.lt b bound)
-      (VARINFOS: forall b gv, Genv.find_var_info ge b = Some gv -> Block.lt b bound).
+      (INIT: inject_incr init_f f)
+      (DOMAIN: forall b, Block.lt b Block.init -> f b = Some(b, 0))
+      (IMAGE: forall b1 b2 delta, f b1 = Some(b2, delta) -> Block.lt b2 Block.init -> b1 = b2)
+      (SYMBOLS: forall id b, Genv.find_symbol ge id = Some b -> Block.lt b Block.init)
+      (FUNCTIONS: forall b fd, Genv.find_funct_ptr ge b = Some fd -> Block.lt b Block.init)
+      (VARINFOS: forall b gv, Genv.find_var_info ge b = Some gv -> Block.lt b Block.init).
 
 Remark inj_preserves_globals:
-  forall f hi,
-  match_globalenvs f hi ->
+  forall f,
+  match_globalenvs f ->
   meminj_preserves_globals ge f.
 Proof.
   intros. inv H.
@@ -446,17 +445,11 @@ Proof.
 Qed.
 
 Lemma match_globalenvs_inject_incr:
-  forall j bound,
-    match_globalenvs j bound ->
-    inject_incr (Mem.flat_inj init_nb) j.
+  forall j,
+    match_globalenvs j ->
+    inject_incr init_f j.
 Proof.
-  inversion 1; subst.
-  unfold inject_incr, Mem.flat_inj.
-  intros.
-  destruct (Block.lt_dec b init_nb); try discriminate.
-  inv H0.
-  eapply DOMAIN.
-  blomega.
+  destruct 1; auto.
 Qed.
 
 (** * Invariant on abstract call stacks  *)
@@ -490,9 +483,9 @@ Definition callstack : Type := list frame.
 Inductive match_callstack (f: meminj) (m: mem) (tm: mem):
                           callstack -> block -> block -> Prop :=
   | mcs_nil:
-      forall hi bound tbound,
-      match_globalenvs f hi ->
-      Block.le hi bound -> Block.le hi tbound ->
+      forall bound tbound,
+      match_globalenvs f ->
+      Block.le Block.init bound -> Block.le Block.init tbound ->
       match_callstack f m tm nil bound tbound
   | mcs_cons:
       forall cenv tf e le te sp lo hi cs bound tbound
@@ -510,7 +503,7 @@ Inductive match_callstack (f: meminj) (m: mem) (tm: mem):
 Lemma match_callstack_match_globalenvs:
   forall f m tm cs bound tbound,
   match_callstack f m tm cs bound tbound ->
-  exists hi, match_globalenvs f hi.
+  match_globalenvs f.
 Proof.
   induction 1; eauto.
 Qed.
@@ -518,7 +511,7 @@ Qed.
 Lemma match_callstack_inject_incr:
   forall f m tm cs bound tbound,
     match_callstack f m tm cs bound tbound ->
-    inject_incr (Mem.flat_inj init_nb) f.
+    inject_incr init_f f.
 Proof.
   intros.
   exploit match_callstack_match_globalenvs; eauto.
@@ -526,8 +519,8 @@ Proof.
   eauto using match_globalenvs_inject_incr.
 Qed.
 
-Lemma match_globalenvs_wf f hi:
-  match_globalenvs f hi ->
+Lemma match_globalenvs_wf f:
+  match_globalenvs f ->
   CKLR.meminj_wf f.
 Proof.
   intros [ ]. split.
@@ -537,8 +530,6 @@ Proof.
   - intros b1 b2 [delta Hb] Hb2.
     assert (b1 = b2); try congruence.
     eapply IMAGE; eauto.
-    eapply Block.lt_le_trans; eauto.
-    eapply Block.le_trans; eauto.
 Qed.
 
 (** Invariance properties for [match_callstack]. *)
@@ -557,6 +548,7 @@ Proof.
   (* base case *)
   econstructor; eauto.
   inv H. constructor; intros; eauto.
+  transitivity f1; eauto.
   eapply IMAGE; eauto. eapply H6; eauto. blomega.
   (* inductive case *)
   assert (Block.le lo hi) by (eapply me_low_high; eauto).
@@ -677,8 +669,9 @@ Proof.
   intros UNMAPPED OUTOFREACH INCR SEPARATED MAXPERMS.
   induction 1; intros.
 (* base case *)
-  apply mcs_nil with hi; auto.
+  apply mcs_nil; auto.
   inv H. constructor; auto.
+  transitivity f1; eauto.
   intros. case_eq (f1 b1).
   intros [b2' delta'] EQ. rewrite (INCR _ _ _ EQ) in H. inv H. eauto.
   intro EQ. exploit SEPARATED; eauto. intros [A B]. elim B. red. blomega.
@@ -1487,7 +1480,7 @@ Proof.
   constructor. simpl. rewrite Ptrofs.add_zero_l; auto.
   congruence.
   (* global *)
-  exploit match_callstack_match_globalenvs; eauto. intros [bnd MG]. inv MG.
+  exploit match_callstack_match_globalenvs; eauto. intros MG. inv MG.
   exists (Vptr b Ptrofs.zero); split.
   constructor. simpl. unfold Genv.symbol_address. 
   rewrite symbols_preserved. rewrite H2. auto.
@@ -1673,10 +1666,10 @@ Inductive match_states: Csharpminor.state -> Cminor.state -> Prop :=
                    (Returnstate tv tk tm).
 
 Remark val_inject_function_pointer_block:
-  forall bound v b fd f tv,
+  forall v b fd f tv,
   block_of v = Some b ->
   Genv.find_funct_ptr ge b = Some fd ->
-  match_globalenvs f bound ->
+  match_globalenvs f ->
   Val.inject f v tv ->
   tv = v.
 Proof.
@@ -1687,9 +1680,9 @@ Proof.
 Qed.
 
 Remark val_inject_function_pointer:
-  forall bound v fd f tv,
+  forall v fd f tv,
   Genv.find_funct ge v = Some fd ->
-  match_globalenvs f bound ->
+  match_globalenvs f ->
   Val.inject f v tv ->
   tv = v.
 Proof.
@@ -2071,7 +2064,7 @@ Proof.
   monadInv TR.
   exploit transl_expr_correct; eauto. intros [tvf [EVAL1 VINJ1]].
   assert (tvf = vf).
-    exploit match_callstack_match_globalenvs; eauto. intros [bnd MG].
+    exploit match_callstack_match_globalenvs; eauto. intros MG.
     eapply val_inject_function_pointer_block; eauto.
   subst tvf.
   exploit transl_exprlist_correct; eauto.
@@ -2087,7 +2080,7 @@ Proof.
   monadInv TR.
   exploit transl_exprlist_correct; eauto.
   intros [tvargs [EVAL2 VINJ2]].
-  exploit match_callstack_match_globalenvs; eauto. intros [hi' MG].
+  exploit match_callstack_match_globalenvs; eauto. intros MG.
   exploit external_call_mem_inject; eauto.
   eapply inj_preserves_globals; eauto.
   intros [f' [vres' [tm' [EC [VINJ [MINJ' [UNMAPPED [OUTOFREACH [INCR SEPARATED]]]]]]]]].
@@ -2242,7 +2235,7 @@ Opaque PTree.set.
 
 (* external call *)
   rewrite FIND in H; inv H. monadInv TR.
-  exploit match_callstack_match_globalenvs; eauto. intros [hi MG].
+  exploit match_callstack_match_globalenvs; eauto. intros MG.
   exploit external_call_mem_inject; eauto.
   eapply inj_preserves_globals; eauto.
   intros [f' [vres' [tm' [EC [VINJ [MINJ' [UNMAPPED [OUTOFREACH [INCR SEPARATED]]]]]]]]].
@@ -2271,14 +2264,14 @@ Require Import Inject.
 Require Import InjectFootprint.
 
 Lemma transl_initial_states:
-  forall w q1 q2, match_query cc_inject_triangle w q1 q2 ->
+  forall w q1 q2, match_query (cc_c inj) w q1 q2 ->
   forall S, Csharpminor.initial_state ge q1 S ->
   exists R,
     Cminor.initial_state tge q2 R /\
     match_states w S R.
 Proof.
-  inv_triangle_query.
-  intros fb sg vargs m0 Hfb Hvargs Hm0 S HS.
+  inv_query_inj.
+  intros f_init id sg vargs1 vargs2 m1 m2 Hvargs Hm INCR IMG S HS.
   inv HS.
   exploit function_ptr_translated; eauto. intros [tf [FIND TR]].
   econstructor; split.
@@ -2286,30 +2279,30 @@ Proof.
   erewrite <- sig_preserved by eauto.
   monadInv TR.
   econstructor; eauto.
-  pose proof (Mem.init_nextblock m0) as Hnb.
-  eapply match_callstate with (f := Mem.flat_inj (Mem.nextblock m0)) (cs := @nil frame) (cenv := PTree.empty Z).
+  eapply match_callstate with (cs := @nil frame) (cenv := PTree.empty Z).
   eauto. eauto.
   auto.
   eauto.
-  apply mcs_nil with (Mem.nextblock m0). econstructor.
-  assumption.
-  apply Block.le_refl.
-  unfold Mem.flat_inj. intros.
-  destruct (Block.lt_dec b (Mem.nextblock m0)); try contradiction. reflexivity.
-  unfold Mem.flat_inj. intros.
-  destruct (Block.lt_dec b1 (Mem.nextblock m0)); congruence.
-  intros. exploit Genv.genv_symb_range; eauto. blomega.
-  intros. apply Genv.find_funct_ptr_iff in H. exploit Genv.genv_defs_range; eauto. blomega.
-  intros. apply Genv.find_var_info_iff in H. exploit Genv.genv_defs_range; eauto. blomega.
-  apply Block.le_refl.
-  apply Block.le_refl.
+  apply mcs_nil; eauto.
+  constructor; eauto.
+  { intros. specialize (INCR b b 0). unfold Mem.flat_inj in INCR.
+    destruct (Block.lt_dec b Block.init); try contradiction. auto. }
+  { intros. specialize (INCR b1 b1 0). unfold Mem.flat_inj in INCR.
+    destruct (Block.lt_dec b1 Block.init).
+    - specialize (INCR eq_refl). congruence.
+    - elim n. eauto. }
+  intros. exploit Genv.genv_symb_range; eauto.
+  intros. apply Genv.find_funct_ptr_iff in H. eapply Genv.genv_defs_range; eauto.
+  intros. apply Genv.find_var_info_iff in H. eapply Genv.genv_defs_range; eauto.
+  apply Mem.init_nextblock.
+  apply Mem.init_nextblock.
   econstructor.
   constructor.
   assumption.
 Qed.
 
 Lemma transl_external:
-  forall (w: ccworld cc_inject_triangle) S R q1,
+  forall w S R q1,
   match_states w S R ->
   Csharpminor.at_external ge S q1 ->
   exists wA q2,
@@ -2326,16 +2319,7 @@ Proof.
   destruct Hq1 as [b id sg vargs1 k1 m1 Hb].
   inv HSR.
   edestruct (match_cc_inject b sg) as (wA & Hq & H); eauto.
-  {
-    eapply match_callstack_match_globalenvs in MCS as (hi & Hge).
-    eapply funct_ptr_flat_inject; eauto.
-    destruct Hge; eauto.
-    eapply match_globalenvs_inject_incr; eauto.
-  }
-  {
-    eapply match_callstack_match_globalenvs in MCS as [hi Hge].
-    eapply match_globalenvs_wf; eauto.
-  }
+  eauto using match_globalenvs_wf, match_callstack_match_globalenvs.
   inv TR.
   assert (fd = External (EF_external id sg)) by congruence; subst fd.
   exists wA, (cq b sg targs tm); repeat apply conj; eauto.
@@ -2359,19 +2343,19 @@ Lemma transl_final_states:
   match_states w S R ->
   Csharpminor.final_state S r1 ->
   exists r2,
-    match_reply cc_inject_triangle w r1 r2 /\
+    match_reply (cc_c inj) w r1 r2 /\
     Cminor.final_state R r2.
 Proof.
   intros. inv H0. inv H. inv MK. inv MCS.
   exists (tv, tm). split.
-  - eapply match_reply_cc_inject_triangle; eauto.
-    eapply match_globalenvs_inject_incr; eassumption.
+  - eapply match_reply_inj; eauto.
+    eapply match_globalenvs_inject_incr; auto.
     eapply match_globalenvs_wf; eauto.
   - constructor.
 Qed. 
 
 Theorem transl_program_correct:
-  forward_simulation (cc_c injp) cc_inject_triangle
+  forward_simulation (cc_c injp) (cc_c inj)
     (Csharpminor.semantics prog)
     (Cminor.semantics tprog).
 Proof.
